code/hash/Hacl.Hash.Core.SHA2.fst
@@ -1,6 +1,6 @@
 module Hacl.Hash.Core.SHA2
 
-module U8 = FStar.UInt8
+open Lib.IntTypes
 module U32 = FStar.UInt32
 module U64 = FStar.UInt64
 module U128 = FStar.UInt128
@@ -50,7 +50,7 @@ let index_h (a: sha2_alg) (i: U32.t): ST.Stack (word a)
   (requires (fun _ -> U32.v i < 8))
   (ensures (fun h0 r h1 ->
     B.(modifies loc_none h0 h1) /\
-    r = S.index (h a) (U32.v i)))
+    r == S.index (h a) (U32.v i)))
 =
     match a with
     | SHA2_224 -> B.recall h224; IB.recall_contents h224 Constants.h224; h224.(i)
@@ -126,13 +126,13 @@ let block_w (a: sha2_alg) =
   b:B.buffer (word a) { B.length b = Helpers.block_word_length }
 
 let block_b (a: sha2_alg) =
-  b:B.buffer U8.t { FStar.Mul.(B.length b = block_word_length * word_length a) }
+  b:B.buffer uint8 { FStar.Mul.(B.length b = block_word_length * word_length a) }
 
 inline_for_extraction
 let ws_w (a: sha2_alg) = b:B.buffer (word a) { B.length b = Spec.size_k_w a }
 
 let block_words_be (a: sha2_alg) (h: HS.mem) (b: block_b a) =
-  words_of_bytes a block_word_length (B.as_seq h b)
+  words_of_bytes a #block_word_length (B.as_seq h b)
 
 inline_for_extraction
 val ws (a: sha2_alg) (b: block_b a) (ws: ws_w a):
@@ -145,19 +145,18 @@ val ws (a: sha2_alg) (b: block_b a) (ws: ws_w a):
       B.as_seq h1 ws == S.init (Spec.size_k_w a) (Spec.ws a b)))
 
 inline_for_extraction
-let index_be (a: sha2_alg) (b: B.buffer U8.t) (i: U32.t):
+let index_be (a: sha2_alg) (b: block_b a) (i: U32.t):
   ST.Stack (word a)
     (requires (fun h ->
-      B.length b % word_length a = 0 /\
       B.live h b /\
-      U32.v i < B.length b / word_length a))
+      U32.v i < block_word_length))
     (ensures (fun h0 r h1 ->
        M.(modifies loc_none h0 h1) /\
-       r = S.index (words_of_bytes a (B.length b / word_length a) (B.as_seq h0 b)) (U32.v i)))
+       r == S.index (words_of_bytes a #(B.length b / word_length a) (B.as_seq h0 b)) (U32.v i)))
 =
   match a with
-  | SHA2_224 | SHA2_256 -> C.Endianness.index_32_be b i
-  | SHA2_384 | SHA2_512 -> C.Endianness.index_64_be b i
+  | SHA2_224 | SHA2_256 -> Lib.ByteBuffer.uint_at_index_be #U32 #SEC #(size block_word_length) b i
+  | SHA2_384 | SHA2_512 -> Lib.ByteBuffer.uint_at_index_be #U64 #SEC #(size block_word_length) b i
 
 #set-options "--max_fuel 1 --z3rlimit 20"
 
@@ -204,7 +203,7 @@ let ws a b ws =
 
       let s1 = Spec._sigma1 a t2 in
       let s0 = Spec._sigma0 a t15 in
-      let w = Spec.word_add_mod a s1 (Spec.word_add_mod a t7 (Spec.word_add_mod a s0 t16)) in
+      let w = s1 +. t7 +. s0 +. t16 in
       ws.(i) <- w;
       (**) let h2 = ST.get () in
       (**) init_next (B.as_seq h2 ws) (Spec.ws a (block_words_be a h0 b)) (U32.v i)
@@ -235,8 +234,6 @@ let k0 a =
       IB.recall_contents k384_512 (S.seq_of_list Constants.k384_512_l);
       k384_512
 
-inline_for_extraction unfold
-let add = Spec.word_add_mod
 
 inline_for_extraction
 val shuffle_core (a: sha2_alg)
@@ -257,7 +254,7 @@ val shuffle_core (a: sha2_alg)
       M.(modifies (loc_buffer hash) h0 h1) /\
       B.as_seq h1 hash == Spec.shuffle_core a b (B.as_seq h0 hash) (U32.v t)))
 
-#set-options "--z3rlimit 50"
+#set-options "--max_fuel 1 --z3rlimit 100"
 inline_for_extraction
 let shuffle_core a block hash ws t =
   let a0 = hash.(0ul) in
@@ -271,14 +268,14 @@ let shuffle_core a block hash ws t =
 
   let w = ws.(t) in
 
-  let t1 = add a h0 (add a (Spec._Sigma1 a e0) (add a (Spec._Ch a e0 f0 g0) (add a (k0 a).(t) w))) in
-  let t2 = add a (Spec._Sigma0 a a0) (Spec._Maj a a0 b0 c0) in
+  let t1 = h0 +. (Spec._Sigma1 a e0) +. (Spec._Ch a e0 f0 g0) +. (k0 a).(t) +. w in
+  let t2 = (Spec._Sigma0 a a0) +. (Spec._Maj a a0 b0 c0) in
 
-  hash.(0ul) <- add a t1 t2;
+  hash.(0ul) <- t1 +. t2;
   hash.(1ul) <- a0;
   hash.(2ul) <- b0;
   hash.(3ul) <- c0;
-  hash.(4ul) <- add a d0 t1;
+  hash.(4ul) <- d0 +. t1;
   hash.(5ul) <- e0;
   hash.(6ul) <- f0;
   hash.(7ul) <- g0;
@@ -286,10 +283,11 @@ let shuffle_core a block hash ws t =
   (**) reveal_opaque (`%Spec.shuffle_core) Spec.shuffle_core;
   (**) let h = ST.get () in
   (**) [@inline_let]
-  (**) let l = [ add a t1 t2; a0; b0; c0; add a d0 t1; e0; f0; g0 ] in
+  (**) let l = [ t1 +. t2; a0; b0; c0; d0 +. t1; e0; f0; g0 ] in
   (**) assert_norm (List.Tot.length l = 8);
   (**) S.intro_of_list #(word a) (B.as_seq h hash) l
 
+#reset-options "--max_fuel 2 --z3rlimit 500"
 inline_for_extraction
 val shuffle: a:sha2_alg -> block:G.erased (block_b a) -> hash:words_state a -> ws:ws_w a ->
   ST.Stack unit
@@ -340,10 +338,10 @@ let shuffle a block hash ws =
 inline_for_extraction
 let zero (a: sha2_alg): word a =
   match a with
-  | SHA2_224 | SHA2_256 -> 0ul
-  | SHA2_384 | SHA2_512 -> 0UL
+  | SHA2_224 | SHA2_256 -> u32 0
+  | SHA2_384 | SHA2_512 -> u64 0
 
-#set-options "--max_fuel 0 --max_ifuel 0"
+#set-options "--z3rlimit 200 --max_fuel 2 --max_ifuel 2"
 
 noextract inline_for_extraction
 val update: a:sha2_alg -> update_st a
@@ -359,9 +357,16 @@ let update a hash block =
   (**) assert (S.equal (B.as_seq h1 hash1) (B.as_seq h0 hash));
   (**) assert (S.equal (B.as_seq h1 hash) (B.as_seq h0 hash));
   shuffle a (G.hide block) hash1 computed_ws;
-  C.Loops.in_place_map2 hash hash1 8ul (add a);
-  (**) ST.pop_frame ();
+  (**) let h2 = ST.get () in
+  (**) assert (let block_w = words_of_bytes a #block_word_length (B.as_seq h1 block) in
+	       S.equal (B.as_seq h2 hash1) (Spec.shuffle a (B.as_seq h1 hash1) block_w));
+  C.Loops.in_place_map2 hash hash1 8ul ( +. );
+  (**) let h3 = ST.get () in
+  (**) reveal_opaque (`%Spec.shuffle) Spec.shuffle;
+  (**) assert (S.equal (B.as_seq h3 hash) (Spec.update_aux a (B.as_seq h1 hash1) (B.as_seq h1 block)));
+  ST.pop_frame();
   (**) reveal_opaque (`%Spec.update) Spec.update
+
 
 let update_224: update_st SHA2_224 = update SHA2_224
 let update_256: update_st SHA2_256 = update SHA2_256
